examples/json/test.fst
@@ -1,0 +1,169 @@
+
+let test
+  (a: int)
+: Tot (
+    (b: int) ->
+    Stack int
+    (requires (fun h -> True))
+    (ensures (fun h res h' -> True))
+  )
+  =
+  fun b -> a + b
+
+(*
+let test
+  (a: int)
+: Pure (
+    (b: int) ->
+    Stack int
+    (requires (fun h -> True))
+    (ensures (fun h res h' -> True))
+  )
+  (True)
+  ((fun _ -> True))
+  =
+  fun b -> a + b
+
+let rec parse_exact_string_contents
+  (against: string)
+: Pure (
+    (b: bstring) -> 
+    (len: UInt32.t) -> 
+    Stack bool
+    (requires (fun h -> string_buffer_valid h b len))
+    (ensures (fun h res h' -> parse_exact_string_contents_postcond against b len h res h'))
+  )
+  (requires True)
+  (ensures (fun v -> True))
+  (decreases (Seq.length against))
+= if
+    Seq.length against = 0
+  then
+    let f
+      (b: bstring)
+      (len: UInt32.t)
+    : Stack bool
+      (requires (fun h -> string_buffer_valid h b len))
+      (ensures (fun h res h' -> parse_exact_string_contents_postcond against b len h res h'))
+    = true
+    in
+    f
+  else
+    let c = Seq.head against in
+    let _ : squash (Seq.length (Seq.tail against) < Seq.length against) = () in
+    let recurse = parse_exact_string_contents (Seq.tail against) in
+    let f
+      (b: bstring)
+      (len: UInt32.t)
+    : Stack bool
+      (requires (fun h -> string_buffer_valid h b len))
+      (ensures (fun h res h' -> parse_exact_string_contents_postcond against b len h res h'))
+    = if
+        len = 0ul
+      then
+        false
+      else if
+        Buffer.index b 0ul = c
+      then
+        let len' = FStar.UInt32.(len -^ 1ul) in
+        let b' = Buffer.sub b 1ul len' in
+        recurse b' len'
+      else
+        false
+    in
+    f
+*)
+
+(* // OK
+let rec parse_exact_string_contents
+  (against: string)
+  (b: bstring)
+  (len: UInt32.t)
+: Stack bool
+  (requires (fun h -> string_buffer_valid h b len))
+  (ensures (fun h res h' -> parse_exact_string_contents_postcond against b len h res h'))
+= if
+    Seq.length against = 0
+  then
+    true
+  else
+    let h = ST.get () in
+    let c = Seq.head against in
+    if
+      len = 0ul
+    then
+      false
+    else if
+      Buffer.index b 0ul = c
+    then
+      let len' = FStar.UInt32.(len -^ 1ul) in
+      let b' = Buffer.sub b 1ul len' in
+      parse_exact_string_contents (Seq.tail against) b' len'
+    else
+      false
+*)
+
+(* // OK
+let rec parse_exact_string_contents
+  (against: string)
+: Tot (
+    (b: bstring) -> 
+    (len: UInt32.t) -> 
+    Stack bool
+    (requires (fun h -> string_buffer_valid h b len))
+    (ensures (fun h res h' -> parse_exact_string_contents_postcond against b len h res h'))
+  )
+= if
+    Seq.length against = 0
+  then
+    let f
+      (b: bstring)
+      (len: UInt32.t)
+    : Stack bool
+      (requires (fun h -> string_buffer_valid h b len))
+      (ensures (fun h res h' -> parse_exact_string_contents_postcond against b len h res h'))
+    = true
+    in
+    f
+  else
+    let c = Seq.head against in
+    let recurse = parse_exact_string_contents (Seq.tail against) in
+    let f
+      (b: bstring)
+      (len: UInt32.t)
+    : Stack bool
+      (requires (fun h -> string_buffer_valid h b len))
+      (ensures (fun h res h' -> parse_exact_string_contents_postcond against b len h res h'))
+    = if
+        len = 0ul
+      then
+        false
+      else if
+        Buffer.index b 0ul = c
+      then
+        let len' = FStar.UInt32.(len -^ 1ul) in
+        let b' = Buffer.sub b 1ul len' in
+        recurse b' len'
+      else
+        false
+    in
+    f
+*)
+
+let rec test2 () : Stack False (requires (fun _ -> True)) (ensures (fun _ _ _ -> False)) = test2 ()
+
+let rec test3 () : Tot (unit ->
+     Stack False (requires (fun _ -> True)) (ensures (fun _ _ _ -> False))) = test3 ()
+
+
+noeq type y = {
+  k: (unit ->
+     Stack False (requires (fun _ -> True)) (ensures (fun _ _ _ -> False)))
+}
+
+(* // KO (as expected)
+let rec test4 () : Tot y
+= test4 ()
+*)
+
+let rec test5 (n: nat) : Tot y = if n = 0 then let r = { k = test3 () } in r else test5 (n-1) 
